More numerically stable softmax, but with significant duplication

dist/Klas_RowSoftmax.cu
@@ -1,6 +1,47 @@
 
 #include "Klas_RowSoftmax.h"
 
+__global__
+/**
+  hoisted when extracting row_softmax_rm_f32
+*/
+static void __hoisted_row_softmax_rm_f32_0(uint32_t n, float *a, float *maxs,
+                                           uint32_t nthm)
+{
+    float *sa1 = (float *)KPR_SHMEM_AT(0U);
+    float acc = a[blockIdx.x * n + threadIdx.x];
+    uint32_t idx = threadIdx.x + nthm;
+    for (; idx < n; idx += nthm)
+        acc = fmaxf(acc, a[blockIdx.x * n + idx]);
+    sa1[threadIdx.x] = acc;
+    uint32_t n1 = 0U;
+    for (; 1U << (uint32_t) n1 < nthm; n1++) {
+        uint32_t __anf01 = n1;
+        __syncthreads();
+        uint32_t nextid = threadIdx.x + (uint32_t) (1U << (uint32_t) __anf01);
+        if (nextid < nthm)
+            if ((threadIdx.x & (uint32_t) (1U << (uint32_t) (__anf01 + 1U)) -
+                 1U) == 0U)
+                sa1[threadIdx.x] = fmaxf(sa1[threadIdx.x], sa1[nextid]);
+    }
+    if (threadIdx.x == 0U)
+        maxs[blockIdx.x] = *sa1;
+}
+
+__global__
+/**
+  hoisted when extracting row_softmax_rm_f32
+*/
+static void __hoisted_row_softmax_rm_f32_1(uint32_t m, uint32_t n, float *a,
+                                           float *maxs)
+{
+    if (1024U * blockIdx.x + threadIdx.x < m * n) {
+        uint32_t row = (1024U * blockIdx.x + threadIdx.x) / n;
+        uint32_t col = (1024U * blockIdx.x + threadIdx.x) % n;
+        a[row * n + col] -= maxs[row];
+    }
+}
+
 typedef struct __uint32_t__uint32_t_______s {
     uint32_t fst;
     uint32_t snd;
@@ -10,7 +51,7 @@ __global__
 /**
   hoisted when extracting row_softmax_rm_f32
 */
-static void __hoisted_row_softmax_rm_f32_0(uint32_t n, float *a, float *sums)
+static void __hoisted_row_softmax_rm_f32_2(uint32_t n, float *a, float *sums)
 {
     float *sa1 = (float *)KPR_SHMEM_AT(0U);
     float acc = 0.0f;
@@ -39,7 +80,7 @@ __global__
 /**
   hoisted when extracting row_softmax_rm_f32
 */
-static void __hoisted_row_softmax_rm_f32_1(uint32_t m, uint32_t n, float *a,
+static void __hoisted_row_softmax_rm_f32_3(uint32_t m, uint32_t n, float *a,
                                            float *sums)
 {
     if (1024U * blockIdx.x + threadIdx.x < m * n) {
@@ -53,25 +94,80 @@ static void __hoisted_row_softmax_rm_f32_1(uint32_t m, uint32_t n, float *a,
 
 void Klas_RowSoftmax_row_softmax_rm_f32(uint32_t m, uint32_t n, float *a)
 {
+    float *maxs = (float *)KPR_GPU_ALLOC(sizeof(float), m);
     float *sums = (float *)KPR_GPU_ALLOC(sizeof(float), m);
-    KPR_SHMEM_FITS(4096U);
+    uint32_t nthm = 1024U <= n ? 1024U : n;
+    KPR_SHMEM_FITS(4U * nthm);
     MUST(cudaFuncSetAttribute(__hoisted_row_softmax_rm_f32_0,
                               cudaFuncAttributeMaxDynamicSharedMemorySize,
-                              4096U));
-    KPR_KCALL(__hoisted_row_softmax_rm_f32_0, m, 1024U, 4096U, n, a, sums);
+                              4U * nthm));
+    KPR_KCALL(__hoisted_row_softmax_rm_f32_0, m, nthm, 4U * nthm, n, a, maxs,
+              nthm);
     MUST(cudaDeviceSynchronize());
     KPR_KCALL(__hoisted_row_softmax_rm_f32_1,
+              m * n / 1024U + (uint32_t) (m * n % 1024U != 0U),
+              1024U, 0U, m, n, a, maxs);
+    MUST(cudaDeviceSynchronize());
+    KPR_SHMEM_FITS(4096U);
+    MUST(cudaFuncSetAttribute(__hoisted_row_softmax_rm_f32_2,
+                              cudaFuncAttributeMaxDynamicSharedMemorySize,
+                              4096U));
+    KPR_KCALL(__hoisted_row_softmax_rm_f32_2, m, 1024U, 4096U, n, a, sums);
+    MUST(cudaDeviceSynchronize());
+    KPR_KCALL(__hoisted_row_softmax_rm_f32_3,
               m * n / 1024U + (uint32_t) (m * n % 1024U != 0U),
               1024U, 0U, m, n, a, sums);
     MUST(cudaDeviceSynchronize());
     MUST(cudaFree(sums));
+    MUST(cudaFree(maxs));
 }
 
 __global__
 /**
   hoisted when extracting row_softmax_rm_f64
 */
-static void __hoisted_row_softmax_rm_f64_0(uint32_t n, double *a, double *sums)
+static void __hoisted_row_softmax_rm_f64_0(uint32_t n, double *a, double *maxs,
+                                           uint32_t nthm)
+{
+    double *sa1 = (double *)KPR_SHMEM_AT(0U);
+    double acc = a[blockIdx.x * n + threadIdx.x];
+    uint32_t idx = threadIdx.x + nthm;
+    for (; idx < n; idx += nthm)
+        acc = fmax(acc, a[blockIdx.x * n + idx]);
+    sa1[threadIdx.x] = acc;
+    uint32_t n1 = 0U;
+    for (; 1U << (uint32_t) n1 < nthm; n1++) {
+        uint32_t __anf01 = n1;
+        __syncthreads();
+        uint32_t nextid = threadIdx.x + (uint32_t) (1U << (uint32_t) __anf01);
+        if (nextid < nthm)
+            if ((threadIdx.x & (uint32_t) (1U << (uint32_t) (__anf01 + 1U)) -
+                 1U) == 0U)
+                sa1[threadIdx.x] = fmax(sa1[threadIdx.x], sa1[nextid]);
+    }
+    if (threadIdx.x == 0U)
+        maxs[blockIdx.x] = *sa1;
+}
+
+__global__
+/**
+  hoisted when extracting row_softmax_rm_f64
+*/
+static void __hoisted_row_softmax_rm_f64_1(uint32_t m, uint32_t n, double *a,
+                                           double *maxs)
+{
+    if (1024U * blockIdx.x + threadIdx.x < m * n) {
+        uint32_t row = (1024U * blockIdx.x + threadIdx.x) / n;
+        uint32_t col = (1024U * blockIdx.x + threadIdx.x) % n;
+        a[row * n + col] -= maxs[row];
+    }
+}
+
+__global__
+/**
+  hoisted when extracting row_softmax_rm_f64
+*/
+static void __hoisted_row_softmax_rm_f64_2(uint32_t n, double *a, double *sums)
 {
     double *sa1 = (double *)KPR_SHMEM_AT(0U);
     double acc = 0.0;
@@ -100,7 +196,7 @@ __global__
 /**
   hoisted when extracting row_softmax_rm_f64
 */
-static void __hoisted_row_softmax_rm_f64_1(uint32_t m, uint32_t n, double *a,
+static void __hoisted_row_softmax_rm_f64_3(uint32_t m, uint32_t n, double *a,
                                            double *sums)
 {
     if (1024U * blockIdx.x + threadIdx.x < m * n) {
@@ -114,16 +210,30 @@ static void __hoisted_row_softmax_rm_f64_1(uint32_t m, uint32_t n, double *a,
 
 void Klas_RowSoftmax_row_softmax_rm_f64(uint32_t m, uint32_t n, double *a)
 {
+    double *maxs = (double *)KPR_GPU_ALLOC(sizeof(double), m);
     double *sums = (double *)KPR_GPU_ALLOC(sizeof(double), m);
-    KPR_SHMEM_FITS(8192U);
+    uint32_t nthm = 1024U <= n ? 1024U : n;
+    KPR_SHMEM_FITS(8U * nthm);
     MUST(cudaFuncSetAttribute(__hoisted_row_softmax_rm_f64_0,
                               cudaFuncAttributeMaxDynamicSharedMemorySize,
-                              8192U));
-    KPR_KCALL(__hoisted_row_softmax_rm_f64_0, m, 1024U, 8192U, n, a, sums);
+                              8U * nthm));
+    KPR_KCALL(__hoisted_row_softmax_rm_f64_0, m, nthm, 8U * nthm, n, a, maxs,
+              nthm);
     MUST(cudaDeviceSynchronize());
     KPR_KCALL(__hoisted_row_softmax_rm_f64_1,
+              m * n / 1024U + (uint32_t) (m * n % 1024U != 0U),
+              1024U, 0U, m, n, a, maxs);
+    MUST(cudaDeviceSynchronize());
+    KPR_SHMEM_FITS(8192U);
+    MUST(cudaFuncSetAttribute(__hoisted_row_softmax_rm_f64_2,
+                              cudaFuncAttributeMaxDynamicSharedMemorySize,
+                              8192U));
+    KPR_KCALL(__hoisted_row_softmax_rm_f64_2, m, 1024U, 8192U, n, a, sums);
+    MUST(cudaDeviceSynchronize());
+    KPR_KCALL(__hoisted_row_softmax_rm_f64_3,
               m * n / 1024U + (uint32_t) (m * n % 1024U != 0U),
               1024U, 0U, m, n, a, sums);
     MUST(cudaDeviceSynchronize());
     MUST(cudaFree(sums));
+    MUST(cudaFree(maxs));
 }
